remove superfluous invariants and add comments

Termination.thy
@@ -44,66 +44,24 @@ definition step where
   "step c c' \<equiv> \<exists> p . receive_step c c' p \<or> daemon_step c c' p"
 
 definition inv1 where
-  "inv1 c \<equiv> \<forall> p . (c\<cdot>visited) p \<or> (\<forall> q . (c\<cdot>S) p q = 0 \<and> (c\<cdot>R) p q = 0)"
+  "inv1 c \<equiv> \<forall> p q . (c\<cdot>R) p q \<le> (c\<cdot>r) p q"
 
 lemma inv1_step:
   assumes "step c c'" and "inv1 c"
   shows "inv1 c'"
 proof -
   have "inv1 c'" if "receive_step c c' p " and "inv1 c" for p
-    using that unfolding receive_step_def inv1_def 
-    by force
-  moreover
-  have "inv1 c'" if "daemon_step c c' p" and "inv1 c" for p
-    using that unfolding daemon_step_def inv1_def 
-    by (auto split:if_splits)
-  ultimately show ?thesis
-    using assms step_def by blast
-qed
-
-definition inv2_a where
-  "inv2_a c \<equiv> \<forall> p q . (c\<cdot>S) p q \<le> (c\<cdot>s) p q"
-
-lemma inv2_a_step:
-  assumes "step c c'" and "inv2_a c"
-  shows "inv2_a c'"
-proof -
-  have "inv2_a c'" if "receive_step c c' p " and "inv2_a c" for p
-    using that unfolding receive_step_def inv2_a_def
-    by (auto; smt (verit, best) trans_le_add1)
-  moreover 
-  have "inv2_a c'" if "daemon_step c c' p " and "inv2_a c" for p
-  proof -
-    have "(c'\<cdot>S) = (c\<cdot>S)(p := (c\<cdot>s) p) \<or> (c'\<cdot>S) = (c\<cdot>S)"
-      using \<open>daemon_step c c' p\<close> unfolding daemon_step_def by (auto split: if_splits)
-    hence "(c'\<cdot>S) = (c\<cdot>S)(p := (c\<cdot>s) p) \<or> (c'\<cdot>S) = (c\<cdot>S)" by blast
-    moreover have "c'\<cdot>s = c\<cdot>s" using \<open>daemon_step c c' p\<close> unfolding daemon_step_def
-      by (auto split:if_splits)
-    ultimately show ?thesis using \<open>inv2_a c\<close> unfolding inv2_a_def by auto
-  qed
-  ultimately show ?thesis
-    using assms step_def by blast
-qed
-
-definition inv2_b where
-  "inv2_b c \<equiv> \<forall> p q . (c\<cdot>R) p q \<le> (c\<cdot>r) p q"
-
-lemma inv2_b_step:
-  assumes "step c c'" and "inv2_b c"
-  shows "inv2_b c'"
-proof -
-  have "inv2_b c'" if "receive_step c c' p " and "inv2_b c" for p
-    using that unfolding receive_step_def inv2_b_def
+    using that unfolding receive_step_def inv1_def
     using nat_le_linear not_less_eq_eq by fastforce
   moreover 
-  have "inv2_b c'" if "daemon_step c c' p" and "inv2_b c" for p
+  have "inv1 c'" if "daemon_step c c' p" and "inv1 c" for p
   proof -
     have "(c'\<cdot>R) = (c\<cdot>R)(p := (c\<cdot>r) p) \<or> (c'\<cdot>R) = (c\<cdot>R)"
       using \<open>daemon_step c c' p\<close> unfolding daemon_step_def by (auto split: if_splits)
     hence "(c'\<cdot>R) = (c\<cdot>R)(p := (c\<cdot>r) p) \<or> (c'\<cdot>R) = (c\<cdot>R)" by blast
     moreover have "c'\<cdot>r = c\<cdot>r" using \<open>daemon_step c c' p\<close> unfolding daemon_step_def
       by (auto split:if_splits)
-    ultimately show ?thesis using \<open>inv2_b c\<close> unfolding inv2_b_def by auto
+    ultimately show ?thesis using \<open>inv1 c\<close> unfolding inv1_def by auto
   qed
   ultimately show ?thesis
     using assms step_def by blast
@@ -136,7 +94,7 @@ definition inv4 where
     \<longrightarrow> (\<exists> p \<in> Q . \<exists> q \<in> -Q . (c\<cdot>r) p q > (c\<cdot>R) p q)"
 
 lemma inv4_step:
-  assumes "step c c'" and "inv1 c" and "inv2_a c" and "inv2_b c" and "inv3 c'" "inv4 c"
+  assumes "step c c'" and "inv1 c" and "inv3 c'" and "inv4 c"
   shows "inv4 c'"
 proof -
   define stale where "stale c Q \<equiv> \<exists> p \<in> Q . \<exists> q . (c\<cdot>R) p q \<noteq> (c\<cdot>r) p q \<or> (c\<cdot>S) p q \<noteq> (c\<cdot>s) p q" for c Q
@@ -153,7 +111,7 @@ proof -
 has received a message from outside Q that the daemon has not seen. This remains true.}\<close> 
           hence "\<exists> p \<in> Q . \<exists> q \<in> -Q . (c\<cdot>r) p q > (c\<cdot>R) p q" using \<open>inv4 c\<close> \<open>consistent c Q\<close> inv4_def stale_def by auto
           hence ?thesis using \<open>receive_step c c' p\<close> unfolding receive_step_def
-            using \<open>inv2_b c\<close> inv2_b_def less_Suc_eq_le by fastforce }
+            using \<open>inv1 c\<close> inv1_def less_Suc_eq_le by fastforce }
         moreover
         { assume "\<not> (stale c Q)"
             \<comment> \<open>If Q is not stale in @{term c}, then no process in Q can receive a message from another process in Q (because all counts match).
@@ -269,7 +227,7 @@ So, because we assume that the count of at least one process in Q changes, it mu
         qed
       next
         case False
-        then show ?thesis 
+        then show ?thesis
           using \<open>daemon_step c c' p\<close> and \<open>consistent c' Q\<close>
             and \<open>stale c' Q\<close>
             and \<open>inv4 c\<close>
